\subsection{具体例}

\subsubsection{$N = 2$ のとき}

\begin{align}
    \tilde{a}_k = \sum_{m = 0}^1 W_2^{mk} a_m
\end{align}

より

偶数のとき

\begin{align*}
    \tilde{a}_k^{e} &= \sum_{m = 0}^0 W_1^{mk} a_{2m} \\
                    &= W_1^0 a_0
\end{align*}

奇数のとき

\begin{align*}
    \tilde{a}_{k}^{o} &= \sum_{m = 0}^0 W_1^{mk} a_{2m + 1} \\
                    &= W_1^0 a_1
\end{align*}

であるので

\begin{align}
    \begin{cases}
        \tilde{a}_0^{e} &= a_0 \\
        \tilde{a}_1^{o} &= a_1 \\
    \end{cases}
\end{align}

ここで

\begin{align*}
    W_2 &= e^{-i\pi} = -1
\end{align*}

であるので

\begin{align}
    \begin{cases}
        \tilde{a}_0 &= a_0 + W_2^0 a_1 = a_0 + a_1 \\
        \tilde{a}_1 &= \tilde{a}_{0 + 2/2} = a_0 - W_2^0 a_1 = a_0 - a_1
    \end{cases}
\end{align}

\subsubsection{$N = 4$ のとき}

\begin{align}
    \tilde{a}_k = \sum_{m = 0}^3 W_4^{mk} a_m
\end{align}

より

偶数のとき

\begin{align*}
    \tilde{a}_k^{e} &= \sum_{m = 0}^1 W_2^{mk} a_{2m}
\end{align*}

奇数のとき

\begin{align*}
    \tilde{a}_{k}^{o} &= \sum_{m = 0}^1 W_2^{mk} a_{2m + 1}
\end{align*}

であるが、それぞれの左辺は $N = 2$ の場合であるので、

\begin{align}
    \begin{cases}
        \tilde{a}_0^{e} &= a_0 + a_2 \\ 
        \tilde{a}_2^{e} &= a_0 - a_2 \\
        \tilde{a}_1^{o} &= a_1 + a_3 \\
        \tilde{a}_3^{o} &= a_1 - a_3
    \end{cases}
\end{align}

ここで

\begin{align}
    \begin{cases}
        \tilde{a}_k &= \tilde{a}_k^{e} + W_4^k \tilde{a}_k^{o} \quad(k = 0,2) \\
        \tilde{a}_{k + 2} &= \tilde{a}_{k + 4/2} = \tilde{a}_k^{o} - W_4^k \tilde{a}_k^{o} \quad (k = 1,3) \\
    \end{cases}
\end{align}

で,$W_4$ は

\begin{align*}
    W_4 &= e^{-i\frac{2\pi}{4}} = -i
\end{align*}

であるので

\begin{align*}
    \tilde{a}_0 &= \tilde{a}_0^e + W_4^0 \tilde{a}_1^o \\
                &= (a_0 + a_2) + (a_1 + a_3) \\
    \tilde{a}_1 &= \tilde{a}_2^e + W_4^1 \tilde{a}_3^o \\
                &= (a_0 - a_2) - i (a_1 - a_3) \\
    \tilde{a}_2 &= \tilde{a}_0^e - W_4^0 \tilde{a}_1^o \\
                &= (a_0 + a_2) - (a_1 + a_3) \\
    \tilde{a}_3 &= \tilde{a}_2^e - W_4^1 \tilde{a}_3^o \\
                &= (a_0 - a_2) + i(a_1 - a_3)
\end{align*}
